optimizations/gt_zero_x.v
@@ -56,11 +56,11 @@ Require Import List.
 Import ListNotations.
 
 
-Module Opt_exp_zero_x.
+Module Opt_gt_zero_x.
 
 
-(* EXP(0,X) = ISZERO(X) *)
-Definition optimize_exp_zero_x_sbinding : opt_smap_value_type := 
+(* GT(0,X) = 0 *)
+Definition optimize_gt_zero_x_sbinding : opt_smap_value_type := 
 fun (val: smap_value) =>
 fun (fcmp: sstack_val_cmp_t) =>
 fun (sb: sbindings) =>
@@ -68,89 +68,95 @@ fun (maxid: nat) =>
 fun (instk_height: nat) =>
 fun (ops: stack_op_instr_map) => 
 match val with
-| SymOp EXP [arg1; arg2] => 
+| SymOp GT [arg1; arg2] => 
   if fcmp arg1 (Val WZero) maxid sb maxid sb instk_height ops then
-    (SymOp ISZERO [arg2], true)
+     (SymBasicVal (Val WZero), true)
   else
     (val, false)
 | _ => (val, false)
 end.
 
 
-Lemma exp_zero_iszero: forall (x: EVMWord) ctx,
-evm_exp ctx [WZero; x] = evm_iszero ctx [x].
-Proof.
-intros. simpl. unfold wordBin. 
-destruct (weqb x WZero) eqn: eq_x_zero.
-- apply weqb_sound in eq_x_zero. rewrite -> eq_x_zero.
-  reflexivity.
-- apply weqb_false in eq_x_zero.
-  rewrite -> N.pow_0_l.
-  + reflexivity.
-  + apply wordToN_neq_0. assumption. 
-Qed.
 
 
 
-Lemma optimize_exp_zero_x_sbinding_smapv_valid:
-opt_smapv_valid_snd optimize_exp_zero_x_sbinding.
+
+Lemma optimize_gt_zero_x_sbinding_smapv_valid:
+opt_smapv_valid_snd optimize_gt_zero_x_sbinding.
 Proof.
 unfold opt_smapv_valid_snd.
 intros instk_height n fcmp sb val val' flag.
-intros Hvalid_smapv_val Hvalid_sb Hoptm_eq_zero_sbinding.
-unfold optimize_exp_zero_x_sbinding in Hoptm_eq_zero_sbinding.
+intros Hvalid_smapv_val Hvalid_sb Hoptm_sbinding.
+unfold optimize_gt_zero_x_sbinding in Hoptm_sbinding.
 destruct (val) as [basicv|pushtagv|label args|offset smem|key sstrg|
-  offset size smem] eqn: eq_val; try inject_rw Hoptm_eq_zero_sbinding eq_val'.
-destruct label eqn: eq_label; try inject_rw Hoptm_eq_zero_sbinding eq_val'.
-(* EXP *)
-destruct args as [|arg1 r1]; try inject_rw Hoptm_eq_zero_sbinding eq_val'.
-destruct r1 as [|arg2 r2]; try inject_rw Hoptm_eq_zero_sbinding eq_val'.
-destruct r2; try inject_rw Hoptm_eq_zero_sbinding eq_val'.
+  offset size smem] eqn: eq_val; try inject_rw Hoptm_sbinding eq_val'.
+destruct label eqn: eq_label; try inject_rw Hoptm_sbinding eq_val'.
+(* GT *)
+destruct args as [|arg1 r1] eqn: eq_args; try 
+  (injection Hoptm_sbinding as eq_val' eq_flag;
+  rewrite <- eq_val'; assumption).
+destruct r1 as [|arg2 r2] eqn: eq_r1; try 
+  (injection Hoptm_sbinding as eq_val' eq_flag;
+  rewrite <- eq_val'; assumption).
+destruct r2 as [|arg3 r3] eqn: eq_r2; try 
+  (injection Hoptm_sbinding as eq_val' eq_flag;
+  rewrite <- eq_val'; assumption).
 destruct (fcmp arg1 (Val WZero) n sb n sb instk_height evm_stack_opm)
-    eqn: eq_fcmp_arg1; try inject_rw Hoptm_eq_zero_sbinding eq_val'.
-injection Hoptm_eq_zero_sbinding as eq_val' eq_flag.
+  eqn: eq_fcmp_arg1; try inject_rw Hoptm_sbinding eq_val'.
+injection Hoptm_sbinding as eq_val' eq_flag.
 rewrite <- eq_val'.
-simpl in Hvalid_smapv_val. unfold valid_stack_op_instr in Hvalid_smapv_val.
-simpl in Hvalid_smapv_val.
-destruct Hvalid_smapv_val as [_ [Hvalid_arg1 [Hvalid_arg2 _]]].
-simpl. unfold valid_stack_op_instr. simpl.
-intuition.
+simpl. intuition.
 Qed.
 
 
-Lemma optimize_exp_zero_x_sbinding_snd:
-opt_sbinding_snd optimize_exp_zero_x_sbinding.
+
+
+Lemma gt_zero_x_zero: forall (x: EVMWord) ctx,
+evm_gt ctx [WZero; x] = WZero.
+Proof.
+intros. simpl. 
+destruct ((wordToN x) <? 0)%N eqn: eq_x_lt_zero.
+- apply N.ltb_lt in eq_x_lt_zero. 
+  pose proof (N.nlt_0_r (wordToN x)) as H.
+  contradiction.
+- reflexivity.
+Qed.
+
+
+Lemma optimize_gt_zero_x_sbinding_snd:
+opt_sbinding_snd optimize_gt_zero_x_sbinding.
 Proof.
 unfold opt_sbinding_snd.
 intros val val' fcmp sb maxidx instk_height idx flag Hsafe_sstack_val_cmp
-  Hvalid Hoptm_eq_zero_sbinding.
+  Hvalid Hoptm_sbinding.
 split.
 - (* valid_sbindings *)
-  apply valid_bindings_snd_opt with (val:=val)(opt:=optimize_exp_zero_x_sbinding)
+  apply valid_bindings_snd_opt with (val:=val)(opt:=optimize_gt_zero_x_sbinding)
     (fcmp:=fcmp)(flag:=flag); try assumption.
-  apply optimize_exp_zero_x_sbinding_smapv_valid. 
+  apply optimize_gt_zero_x_sbinding_smapv_valid. 
     
 - (* evaluation is preserved *) 
   intros stk mem strg ctx v Hlen Heval_orig.
   assert (Hlen2 := Hlen).
   rewrite -> Hlen in Hlen2.
   rewrite <- Hlen in Hlen2 at 2.
-  unfold optimize_exp_zero_x_sbinding in Hoptm_eq_zero_sbinding.
+  unfold optimize_gt_zero_x_sbinding in Hoptm_sbinding.
   pose proof (Hvalid_maxidx instk_height maxidx idx val sb evm_stack_opm
       Hvalid) as eq_maxidx_idx.
   destruct val as [vv|vv|label args|offset smem|key sstrg|offset seze smem]
-    eqn: eq_val; try inject_rw Hoptm_eq_zero_sbinding eq_val'.
+    eqn: eq_val; try inject_rw Hoptm_sbinding eq_val'.
   (* SymOp label args *)
-  destruct label; try inject_rw Hoptm_eq_zero_sbinding eq_val'.
+  destruct label; try inject_rw Hoptm_sbinding eq_val'.
   destruct args as [|arg1 r1] eqn: eq_args; 
-    try inject_rw Hoptm_eq_zero_sbinding eq_val'.
+    try inject_rw Hoptm_sbinding eq_val'.
   destruct r1 as [|arg2 r2] eqn: eq_r1; 
-    try inject_rw Hoptm_eq_zero_sbinding eq_val'.
-  destruct r2; try inject_rw Hoptm_eq_zero_sbinding eq_val'.
+    try inject_rw Hoptm_sbinding eq_val'.
+  destruct r2 as [|arg3 r3] eqn: eq_r2; 
+    try inject_rw Hoptm_sbinding eq_val'.
   destruct (fcmp arg1 (Val WZero) idx sb idx sb instk_height) 
-    eqn: fcmp_arg1_zero; try inject_rw Hoptm_eq_zero_sbinding eq_val'.
-  (* arg1 ~ WZero *)
-  injection Hoptm_eq_zero_sbinding as eq_val' _. 
+    eqn: fcmp_arg1_zero; try inject_rw Hoptm_sbinding eq_val'.
+  (* arg2 ~ WZero *)
+  injection Hoptm_sbinding as eq_val' _. 
   rewrite <- eq_val'.
   unfold eval_sstack_val in Heval_orig. simpl in Heval_orig.
   rewrite -> PeanoNat.Nat.eqb_refl in Heval_orig.
@@ -159,7 +165,6 @@ split.
     as [varg1|] eqn: eval_arg1; try discriminate.
   destruct (eval_sstack_val' maxidx arg2 stk mem strg ctx idx sb evm_stack_opm)
     as [varg2|] eqn: eval_arg2; try discriminate.
-  unfold safe_sstack_val_cmp in Hsafe_sstack_val_cmp.
 
   unfold valid_bindings in Hvalid.
   destruct Hvalid as [eq_maxid [Hvalid_smap_value Hvalid_bindings_sb]].
@@ -174,25 +179,22 @@ split.
     instk_height evm_stack_opm Hvalid_arg1 Hvalid_zero Hvalid_bindings_sb
     Hvalid_bindings_sb fcmp_arg1_zero stk mem strg ctx Hlen2)
     as [vzero [Heval_arg1 Heval_vzero]].
-  assert (Heval_arg1_copy := Heval_arg1).
-  unfold eval_sstack_val in Heval_arg1_copy.
   rewrite -> eval_sstack_val_const in Heval_vzero.
   rewrite <- Heval_vzero in Heval_arg1.
     
-  unfold eval_sstack_val.
-  rewrite -> eq_maxid in eval_arg1.
-  rewrite -> Heval_arg1_copy in eval_arg1.
+  unfold eval_sstack_val in Heval_arg1.
+  rewrite -> eq_maxidx_idx in Heval_arg1.
+  rewrite -> Heval_arg1 in eval_arg1.
   injection eval_arg1 as eq_varg1.
-  injection Heval_vzero as eq_vzero.
   rewrite <- eq_varg1 in Heval_orig.
-  rewrite <- eq_vzero in Heval_orig.
-  simpl. rewrite -> PeanoNat.Nat.eqb_refl.
-  simpl. rewrite -> eval_arg2. 
+  rewrite -> gt_zero_x_zero in Heval_orig.
   rewrite <- Heval_orig.
-    
-  rewrite -> exp_zero_iszero.
+
+  unfold eval_sstack_val.
+  simpl.
+  rewrite -> PeanoNat.Nat.eqb_refl. simpl.
   reflexivity.
 Qed.
 
 
-End Opt_exp_zero_x.
+End Opt_gt_zero_x.
