optimizations/lt_x_one.v
@@ -56,11 +56,11 @@ Require Import List.
 Import ListNotations.
 
 
-Module Opt_gt_one.
+Module Opt_lt_x_one.
 
 
-(* GT(1,X) = ISZERO(X) *)
-Definition optimize_gt_one_sbinding : opt_smap_value_type := 
+(* LT(X,1) = ISZERO(X) *)
+Definition optimize_lt_x_one_sbinding : opt_smap_value_type := 
 fun (val: smap_value) =>
 fun (fcmp: sstack_val_cmp_t) =>
 fun (sb: sbindings) =>
@@ -68,9 +68,9 @@ fun (maxid: nat) =>
 fun (instk_height: nat) =>
 fun (ops: stack_op_instr_map) => 
 match val with
-| SymOp GT [arg1; arg2] => 
-  if fcmp arg1 (Val WOne) maxid sb maxid sb instk_height ops then
-    (SymOp ISZERO [arg2], true)
+| SymOp LT [arg1; arg2] => 
+  if fcmp arg2 (Val WOne) maxid sb maxid sb instk_height ops then
+    (SymOp ISZERO [arg1], true)
   else
     (val, false)
 | _ => (val, false)
@@ -81,44 +81,30 @@ end.
 
 
 
-Lemma optimize_gt_one_sbinding_smapv_valid:
-opt_smapv_valid_snd optimize_gt_one_sbinding.
+Lemma optimize_lt_x_one_sbinding_smapv_valid:
+opt_smapv_valid_snd optimize_lt_x_one_sbinding.
 Proof.
 unfold opt_smapv_valid_snd.
 intros instk_height n fcmp sb val val' flag.
 intros Hvalid_smapv_val Hvalid_sb Hoptm_sbinding.
-unfold optimize_gt_one_sbinding in Hoptm_sbinding.
+unfold optimize_lt_x_one_sbinding in Hoptm_sbinding.
 destruct (val) as [basicv|pushtagv|label args|offset smem|key sstrg|
-  offset size smem] eqn: eq_val; try (
-    injection Hoptm_sbinding as eq_val' eq_flag;
-    rewrite <- eq_val';
-    assumption).
-destruct label eqn: eq_label; try 
-      (injection Hoptm_sbinding as eq_val' eq_flag;
-      rewrite <- eq_val'; assumption).
-(* GT *)
-destruct args as [|arg1 r1] eqn: eq_args; try 
-  (injection Hoptm_sbinding as eq_val' eq_flag;
-  rewrite <- eq_val'; assumption).
-destruct r1 as [|arg2 r2] eqn: eq_r1; try 
-  (injection Hoptm_sbinding as eq_val' eq_flag;
-  rewrite <- eq_val'; assumption).
-destruct r2 as [|arg3 r3] eqn: eq_r2; try 
-  (injection Hoptm_sbinding as eq_val' eq_flag;
-  rewrite <- eq_val'; assumption).
-destruct (fcmp arg1 (Val WOne) n sb n sb instk_height evm_stack_opm)
-  eqn: eq_fcmp_arg1.
-* injection Hoptm_sbinding as eq_val' eq_flag.
-  rewrite <- eq_val'.
-  simpl in Hvalid_smapv_val. unfold valid_stack_op_instr in Hvalid_smapv_val.
-  simpl in Hvalid_smapv_val.
-  destruct Hvalid_smapv_val as [_ [Hvalid_arg1 [Hvalid_arg2 _]]].
-  simpl.
-  unfold valid_stack_op_instr. simpl.
-  intuition.
-* injection Hoptm_sbinding as eq_val' eq_flag.
-  rewrite <- eq_val'.
-  assumption.
+  offset size smem] eqn: eq_val; try inject_rw Hoptm_sbinding eq_val'.
+destruct label eqn: eq_label; try inject_rw Hoptm_sbinding eq_val'.
+(* LT *)
+destruct args as [|arg1 r1]; try inject_rw Hoptm_sbinding eq_val'.
+destruct r1 as [|arg2 r2]; try inject_rw Hoptm_sbinding eq_val'.
+destruct r2 as [|arg3 r3]; try inject_rw Hoptm_sbinding eq_val'. 
+destruct (fcmp arg2 (Val WOne) n sb n sb instk_height evm_stack_opm)
+  eqn: eq_fcmp_arg2; try inject_rw Hoptm_sbinding eq_val'.
+injection Hoptm_sbinding as eq_val' eq_flag.
+rewrite <- eq_val'.
+simpl in Hvalid_smapv_val. unfold valid_stack_op_instr in Hvalid_smapv_val.
+simpl in Hvalid_smapv_val.
+destruct Hvalid_smapv_val as [_ [Hvalid_arg1 [Hvalid_arg2 _]]].
+simpl.
+unfold valid_stack_op_instr. simpl.
+intuition.
 Qed.
 
 
@@ -143,25 +129,38 @@ intros. simpl. destruct ((wordToN x <? 1)%N) eqn: H1.
   reflexivity.
 Qed.
 
+Lemma evmgt_evmlt: forall (x y: EVMWord) ctx,
+evm_gt ctx [x;y] = evm_lt ctx [y;x].
+Proof.
+intros. unfold evm_gt. reflexivity.
+Qed.
 
-Lemma optimize_gt_one_sbinding_snd:
-opt_sbinding_snd optimize_gt_one_sbinding.
+Lemma lt_iszero: forall (x: EVMWord) ctx,
+evm_lt ctx [x; WOne] = evm_iszero ctx [x].
+Proof.
+intros. rewrite <- evmgt_evmlt. 
+apply gt_iszero. 
+Qed.
+
+
+Lemma optimize_lt_x_one_sbinding_snd:
+opt_sbinding_snd optimize_lt_x_one_sbinding.
 Proof.
 unfold opt_sbinding_snd.
 intros val val' fcmp sb maxidx instk_height idx flag Hsafe_sstack_val_cmp
   Hvalid Hoptm_sbinding.
 split.
 - (* valid_sbindings *)
-  apply valid_bindings_snd_opt with (val:=val)(opt:=optimize_gt_one_sbinding)
+  apply valid_bindings_snd_opt with (val:=val)(opt:=optimize_lt_x_one_sbinding)
     (fcmp:=fcmp)(flag:=flag); try assumption.
-  apply optimize_gt_one_sbinding_smapv_valid. 
+  apply optimize_lt_x_one_sbinding_smapv_valid. 
     
 - (* evaluation is preserved *) 
   intros stk mem strg ctx v Hlen Heval_orig.
   assert (Hlen2 := Hlen).
   rewrite -> Hlen in Hlen2.
   rewrite <- Hlen in Hlen2 at 2.
-  unfold optimize_gt_one_sbinding in Hoptm_sbinding.
+  unfold optimize_lt_x_one_sbinding in Hoptm_sbinding.
   pose proof (Hvalid_maxidx instk_height maxidx idx val sb evm_stack_opm
       Hvalid) as eq_maxidx_idx.
   destruct val as [vv|vv|label args|offset smem|key sstrg|offset seze smem]
@@ -174,8 +173,8 @@ split.
     try inject_rw Hoptm_sbinding eq_val'.
   destruct r2 as [|arg3 r3] eqn: eq_r2; 
     try inject_rw Hoptm_sbinding eq_val'.
-  destruct (fcmp arg1 (Val WOne) idx sb idx sb instk_height) 
-    eqn: fcmp_arg1_one.
+  destruct (fcmp arg2 (Val WOne) idx sb idx sb instk_height) 
+    eqn: fcmp_arg2_one.
   + (* arg2 ~ WOne *)
     injection Hoptm_sbinding as eq_val' _. 
     rewrite <- eq_val'.
@@ -197,25 +196,27 @@ split.
 
     pose proof (valid_sstack_value_const instk_height idx v) as 
       Hvalid_one.
-    pose proof (Hsafe_sstack_val_cmp arg1 (Val WOne) idx sb idx sb 
-      instk_height evm_stack_opm Hvalid_arg1 Hvalid_one Hvalid_bindings_sb
-      Hvalid_bindings_sb fcmp_arg1_one stk mem strg ctx Hlen2)
-      as [vone [Heval_arg1 Heval_vone]].
+    pose proof (Hsafe_sstack_val_cmp arg2 (Val WOne) idx sb idx sb 
+      instk_height evm_stack_opm Hvalid_arg2 Hvalid_one Hvalid_bindings_sb
+      Hvalid_bindings_sb fcmp_arg2_one stk mem strg ctx Hlen2)
+      as [vone [Heval_arg2 Heval_vone]].
+    (*assert (Heval_arg2_copy := Heval_arg2).
+    unfold eval_sstack_val in Heval_arg1_copy.*)
     rewrite -> eval_sstack_val_const in Heval_vone.
-    rewrite <- Heval_vone in Heval_arg1.
+    rewrite <- Heval_vone in Heval_arg2.
     
-    unfold eval_sstack_val in Heval_arg1.
-    rewrite -> eq_maxidx_idx in Heval_arg1.
-    rewrite -> Heval_arg1 in eval_arg1.
-    injection eval_arg1 as eq_varg1.
-    rewrite <- eq_varg1 in Heval_orig.
-    rewrite -> gt_iszero in Heval_orig.
+    unfold eval_sstack_val in Heval_arg2.
+    rewrite -> eq_maxidx_idx in Heval_arg2.
+    rewrite -> Heval_arg2 in eval_arg2.
+    injection eval_arg2 as eq_varg2.
+    rewrite <- eq_varg2 in Heval_orig.
+    rewrite -> lt_iszero in Heval_orig.
     rewrite <- Heval_orig.
 
     unfold eval_sstack_val.
     simpl.
     rewrite -> PeanoNat.Nat.eqb_refl. simpl.
-    rewrite -> eval_arg2.
+    rewrite -> eval_arg1.
     reflexivity.
   + injection Hoptm_sbinding as eq_val' _.
     rewrite <- eq_val'.
@@ -223,4 +224,4 @@ split.
 Qed.
 
 
-End Opt_gt_one.
+End Opt_lt_x_one.
